A closed form formula is a recurrence relation which is defined in terms of just n instead of functions within functions like M(n) = 2M(n-1) + 1. Proof by induction is showing that a closed form formula is actually correct - **you prove that the closed form gives the same value as your recurrence relation for all n**. 

Example of induction:
Base step: M(1) = 1
Recursive / inductive step: M(n+1) = 2*M(n-1) + 1

First you want to prove the base step: M(1) = 2^1 - 1
For the inductive step: Assume M(n) works (for some particular n). In this case we will prove M(n+1) = 2^(n+1) - 1; we know M(n+1) = 2M(n) + 1 => M(n) = 2^n - 1 therefore 2*M(n) + 1 = 2 (2^n - 1) + 1 = 2(2^n - 1) + 1 = 2^n+1 - 1