### Textbook Questions: Section 1.1
Exercises: 1, 2, 4, 5, 6, 9, 10, 11, 14, 18, 19, 20, 22, 23, 26, 27.

### Takeaways:
For statement (p) to be *stronger* than another (q), if q is true whenever p is true but not conversely. p -> q is always/more true, but q -> p is not/less. 

##### 1
p = "There is water in the cylinders"
q = "The head gasket is blown"
r = "The car will start"

a. (q -> p) ^ (p -> r)

b. If the car will start then there is either no water in the cyliders or the head gasket is not blown

##### 2
p = "You are in Seoul"
q = "You are in Kwangju"
r = "You are in South Korea"

a. ¬r -> ¬(p v q)

b. If you are in Kwangju, then you are in South Korea and you are not in Seoul

##### 4
s = "If you are studying hard, then you are staying up late at night"

s in formarl logic:
p = "You are studying hard"
q = "You are staying up late at night"
s = p -> q

The converse is when you switch your variables around i.e. q -> p
a. Converse: q -> p

b. Contrapositive: ¬p -> ¬q, nope it's this relationships AND variables are reversed: **¬q -> ¬p**

##### 5
s = "If it is raining, then the ground is wet"
p = "It is raining"
q = "The ground is wet"
s = p -> q 

a. Converse of s: q -> p

b. Contrapositive: ¬q -> ¬p

##### 6
Show that the *converse* of the following statement is false
s = "If a quadrilateral has a pair of parallel sides, then it has a pair of supplementary angles
p = "Quadrilateral has a pair of parallel sides"
q = "Has a pair of supplementary angles"
s = p -> q

q -> p
|p|q|q -> p|
|-|-|:----:|
|T|T|T|
|T|F|T|
|**F**|**T**|**F**|
|F|F|T|

##### 9
Show that p <-> q is logically equivalent to (p -> q) ^ (q -> p)

|p|q|p -> q|q -> p|(p -> q) ^ (q -> p)|p <-> q|
|-|-|:----:|:----:|:-----------------:|:-----:|
|T|T|T|T|T|T|
|T|F|F|T|F|F|
|F|T|T|F|F|F|
|F|F|T|T|T|T|

##### 10
Use truth tables to show the equivalences between:

a. ¬(p v q) equivalent to ¬p ^ ¬q

|p|q|¬p|¬q|p v q|¬p ^ ¬q|¬(p v q)|
|-|-|:-:|:-:|:-:|:-----:|:------:|
|T|T|F|F|T|F|F|
|T|F|F|T|T|F|F|
|F|T|T|F|T|F|F|
|F|F|T|T|F|T|T|

b. ¬(p ^ q) == ¬p v ¬q

|p|q|¬p|¬q|p ^ q|¬p v ¬q|¬(p ^ q)|
|-|-|:-:|:-:|:-:|:-----:|:------:|
|T|T|F|F|T|F|F|
|T|F|F|T|F|T|T|
|F|T|T|F|F|T|T|
|F|F|T|T|F|T|T|

##### 11

?¬(p -> q) == ¬p -> ¬q? Show using truth tables
|p|q|¬p|¬q|p -> q|¬p -> ¬q| ¬(p -> q)|
|-|-|:-:|:-:|:--:|:------:|:--------:|
|T|T|F|F|T|T|F|
|T|F|F|T|F|T|T|
|F|T|T|F|T|F|F|
|F|F|T|T|T|T|F|

They are not equivalent, but in fact opposites.

##### 14
p = "Andy is hungry"
q = "The refrigerator is empty"
r = "Andy is mad"

a. (p ^ q) -> r

b. Truth table:

|p|q|r|p ^ q|(p ^ q) -> r|
|-|-|-|:---:|:----------:|
|T|T|T|T|T|
|T|T|F|T|F|
|T|F|T|F|T|
|T|F|F|F|T|
|F|T|T|F|T|
|F|T|F|F|T|
|F|F|T|F|T|
|F|F|F|F|T|

c. If the statement is true, but Andy is not mad and the fridge is not empty, is he hungry?
He can be either hungry or not hungry since p ^ q.

##### 18
a
b
p = a ^ b
q = a v b
r = a -> b

a. Show a ^ b > a

|b|a|a ^ b|
|-|-|:---:|
|T|T|T|
|T|F|F|
|F|T|F|
|F|F|F|

a is always true when a ^ b is true, but not vice versa

b. Show a > a v b

|b|a|a v b|
|-|-|:---:|
|T|T|T|
|T|F|T|
|F|T|T|
|F|F|F|

a v b is always true when a is true, but not vice versa

c. Show a ^ b  > a v b
|b|a|a v b|a ^ b|
|-|-|:---:|:---:|
|T|T|T|T|
|T|F|T|F|
|F|T|T|F|
|F|F|F|F|

a v b is always true when a ^ b is true, but not vice versa

d. Show b > a -> b

|a|b|a -> b|
|-|-|:----:|
|T|T|T|
|T|F|F|
|F|T|T|
|F|F|T|

a -> b is always true when b is true, but not vice versa

##### 19
Suppose Q is a quadrilateral. Which statement is stronger?
Q is a square || Q is a rectangle
So this would have to be where one is true while the other true and while the other is not true where the first is true. 

All squares are rectangles but not all rectangles are squares therefore, rectangles are stronger.

##### 20
Which statement is stronger?

a = "Manchester United is the best football team in England."
b = "Manchester United is the best football team in Europe."

England is always in Europe but not every team in Europe is in England therefore b is stronger

##### 22
Uhh, idk

##### 23
Nah

##### 26
S = (p ^ q) v (p ^ ¬q)
a. Truth table

|p|q|¬q|p ^ q|p ^ ¬q|(p ^ q) v (p ^ ¬q)|
|-|-|:-:|:--:|:----:|:----------------:|
|T|T|F|T|F|T|
|T|F|T|F|T|T|
|F|T|F|F|F|F|
|F|F|T|F|F|F|

b. Find a simpler expression that is logically equivalent
idk, probably something with demorgan's law or using other symbols or factoring

##### 27
S = [¬(p -> q)] v [¬(p v q)]

a. Truth table
|p|q|p v q|p -> q|¬(p v q)|¬(p -> q)|[¬(p -> q)] v [¬(p v q)]|
|-|-|:---:|:----:|:------:|:-------:|:----------------------:|
|T|T|T|T|F|F|F|
|T|F|F|F|T|T|T|
|F|T|F|T|T|F|T|
|F|F|F|T|T|F|T|

b. Find a simpler expression
¬(p v q) == ¬p ^ ¬q

¬(p -> q) == ?